solved

Exam/Exercise1.dfy
@@ -1,53 +1,124 @@
+// Exercise 1: [6pts]
+// We want to check if an array w is a "slipped version" of another array v of
+// the same length. We say that w is a "slipped version" of v at index k if
+// v[0] == w[k] and the sequence of elements are the same in both arrays
+// considering w as circular: v[1] == w[k+1], v[2] == w[k+2], etc.
+// As example: given v = [2,5,1,6,8] and w= [6,8,2,5,1], w is a slipped version
+// of v at index 2 as v[0] == w[2], v[1] == w[3], v[2] == w[4], v[3] == w[0] and
+// v[4] == w[1].
+// We will solve the problem for arrays where all the elements are different.
 
-//EXERCISE 1: 6 points
-//We want to check if an array w is a "slipped version" of another array v of the same Length
-//We say that w is a slipped version of v at index k if v[0]==w[k] and the sequence of elements
-//are the same in both arrays considering w as circular v[1]==w[k+1], v[2]==w[k+2]....etc
-// As example : given v=[2,5,1,6,8] and w=[6,8,2,5,1], w is a slipped version of v at index 2
-// as v[0]==w[2], v[1]==w[3], v[2]==w[4], v[3]==w[0] and v[4]==w[1]
-//We will solve the problem for arrays where all the elements are different.
+// 1. [0.5pts] Define the following predicates 
+predicate different(v:array<int>)
+reads v {
+    forall i, j :: 0 <= i < j < v.Length ==> v[i] != v[j]
+}
 
-//1. [0.5pt] Define the following predicates 
-predicate different(v : array<int>) 
- reads v;
-//All the elements in v are different
+predicate slipped(v:array<int>, w:array<int>, k:int)
+requires 0 <= k < v.Length == w.Length
+reads v, w {
+    forall i :: 0 <= i < v.Length ==> v[i] == w[(k+i)%w.Length]
+}
 
-predicate slipped(v : array<int>,w : array<int>, k:int)
- requires v.Length == w.Length && 0 <= k < v.Length
- reads v,w
- //The elements of v and w are the same starting at index k: 
- //v[0]==w[k] and so on circularly on w
- //Hint: use %
+predicate slippedUpTo(v:array<int>, w:array<int>, k:int, i:int)
+requires 0 <= k < v.Length == w.Length
+requires 0 <= i <= v.Length == w.Length
+reads v, w {
+    forall j :: 0 <= j < i ==> v[j] == w[(k+j)%w.Length]
+}
 
+lemma slippedUpToTheEnd(v:array<int>, w:array<int>, k:int)
+requires 0 <= k < v.Length == w.Length
+ensures slipped(v, w, k) <==> slippedUpTo(v, w, k, v.Length) {}
 
-//2.[1.5pts] Prove the following lemmas
+// 2. [1.5pts] Prove the following lemmas
+// 2.1. If v[0] is not in w then w is not a slipped version of v for any k
+lemma necessarySlippedCondition(v:array<int>, w:array<int>)
+requires 0 < v.Length == w.Length
+ensures forall kp :: 0 <= kp < v.Length ==>
+    (slipped(v, w, kp) ==> v[0] == w[kp]) {}
+
+lemma firstMustAppear(v:array<int>, w:array<int>)
+requires 0 < v.Length == w.Length
+requires forall k :: 0 <= k < v.Length ==> v[0] != w[k]
+ensures forall k :: 0 <= k < v.Length ==> !slipped(v, w, k) {
+    necessarySlippedCondition(v, w);
+}
  
-//2.1 If v[0] is not in w then w is not a slipped version of v for any k
- lemma firstMustAppear(v:array<int>, w:array<int>)
- requires v.Length>=0 && w.Length==v.Length
- requires (forall k:: 0 <= k < v.Length ==> v[0] != w[k]) 
- ensures  (forall k:: 0 <= k < v.Length ==> !slipped(v,w,k))
- 
-//2.2 If v[0]==w[i] but w is not a slipped version of v at index i
-//then there is no other possibility of being a slipped version of v
-  
-  lemma onlyPossibility(v:array<int>, w:array<int>,i:int)
-   requires v.Length>0 && w.Length==v.Length && 0<=i<v.Length && different(v) && different(w) && v[0]==w[i]
-   requires !slipped(v,w,i)
-   ensures (forall k:: 0 <= k < v.Length ==> !slipped(v,w,k))
+// 2.2. If v[0] == w[k] but w is not a slipped version of v at index k then
+// there is no other possibility of being a slipped version of v
+lemma onlyPossibility(v:array<int>, w:array<int>, k:int)
+requires 0 < v.Length == w.Length
+requires 0 <= k < v.Length
+requires different(v)
+requires different(w)
+requires v[0] == w[k]
+requires !slipped(v, w, k)
+ensures forall kp :: 0 <= kp < v.Length ==> !slipped(v, w, kp) {
+    necessarySlippedCondition(v, w);
+    assert forall i :: 0 <= i < v.Length && i != k ==> v[0] == w[k] != w[i];
+    assert forall kp :: 0 <= kp < v.Length && kp != k ==> !slipped(v, w, kp);
+}
    
-//3.[1 pts] Write the postcondition of method mslipped
-// b is true if and only if w is a slipped version of v
-// If b is true then w is a slipped version of v from index i
-// If b is false i must b v.Length  
+// 3. [1pts] Write the postcondition of method mslipped, i.e., b is true if and
+// only if w is a slipped version of v; if b is true then w is a slipped version
+// of v from index k; and if b is false k must b v.Length
 
-method mslipped(v : array<int>,w : array<int>) returns (b : bool,i:int)
-	requires v.Length > 0 && v.Length==w.Length && different(v) && different(w)
+// 4. [3pts] Implement and verify the method that given two arrays v and w
+// containing different elements checks if w is a slipped version of v. First
+// write a loop for looking for v[0] in w. If it does not appear then w cannot
+// be a slipped version of v. Otherwise if v[0] == w[i], write a loop to check
+// circularly the rest of elements. Use the previous lemmas to verify
 
+method mslipped(v:array<int>, w:array<int>) returns (b:bool, k:int)
+requires 0 < v.Length == w.Length
+requires different(v)
+requires different(w)
+ensures b <==> exists kp :: 0 <= kp < v.Length && slipped(v, w, kp)
+ensures b ==> (0 <= k < v.Length && slipped(v, w, k))
+ensures !b ==> k == v.Length {
+    // First we want to find a candidate for the slipped index k, so we
+    // iterate until we find a k such that v[0] == w[k]. If such k doesn't
+    // exist, then we know that b must be false.
+    k := 0;
+    while k < v.Length && v[0] != w[k]
+    decreases v.Length - k
+    invariant 0 <= k <= v.Length
+    invariant forall i :: 0 <= i < k ==> v[0] != w[i] {
+        k := k + 1;
+    }
+    assert forall i :: 0 <= i < k ==> v[0] != w[i];
+    assert k < v.Length ==> v[0] == w[k];
+    if k == v.Length {
+        assert forall i :: 0 <= i < v.Length ==> v[0] != w[i];
+        firstMustAppear(v, w);
+        b := false;
+        return;
+    }
 
-//4. [3 pts] Implement and verify the method that given two arrays v and w containing different elements
-//checks if w is a slipped version of v
-//First write a loop for looking v[0] in w. If it does not appear then w cannot be a slipped version of v.
-//Otherwise if v[0]==w[i], write a loop to check circularly the rest of elements
-//Use the previous lemmas to verify
+    // We know that if w is a slipped version of v, then it has to be of index k
+    assert k < v.Length && v[0] == w[k];
+    assert forall kp :: 0 <= kp < v.Length && kp != k ==> !slipped(v, w, kp);
 
+    // Now we want to check whether or not w is a slipped version of v of index
+    // k, to do that we simply check if v[i] == w[(k+i)%w.Length] for all
+    // possible index i
+    b := true;
+    var i:int := 0;
+    while i < v.Length && b
+    decreases v.Length - i
+    invariant 0 <= i <= v.Length
+    invariant b <==> slippedUpTo(v, w, k, i)
+    invariant !b ==> (i > 0 && slippedUpTo(v, w, k, i-1)) {
+        if v[i] != w[(k+i)%w.Length] {
+            b := false;
+        }
+        i := i + 1;
+    }
+    assert b ==> slippedUpTo(v, w, k, v.Length);
+    slippedUpToTheEnd(v, w, k);
+    if !b {
+        k := v.Length;
+        return;
+    }
+}
